Logic/Logic/Context.lean
@@ -1,0 +1,7 @@
+import Logic.Logic.System
+
+namespace LO
+
+variable (F S : Type*) [System F S]
+
+end LO
